

The Geometry of Elliptic Curves

1 Projective space

Definition 1.1. Let K be a field and E_K a vector space over K . We denote the *projective space* $P(E_K)$ by

$$P(E_K) = (E - \{0\})/K^\times.$$

Suppose E finite dimension $n < \infty$. Then we have $E \simeq K^n$, which implies

$$P(E_K) \simeq (K^n - \{0\})/K^\times.$$

We observe that two nonzero vectors $u, v \in K^n$ are equivalent, i.e. $u \sim v$, if there exists some $\lambda \in K^\times$ such that $u = \lambda v$. In other words, the points in $P(E_K)$ are given by equivalence classes

$$[u] = Ku = \{\lambda u : \lambda \in K^\times\}.$$

which are one dimensional subspaces spanned by the respective vectors u . We note also that $\dim P(E) = \dim(E_K) - 1$.

Example 1. The space $P(\mathbb{R}^2)$ is given by all the lines in \mathbb{R}^2 , which can be identified with S^1 . Observe here that we have the freedom to choose the point at infinity. Given a chart, we can carry out computations there.

This idea of projectivization will play an important role in the next section when we obtain a projective variety from an affine variety.

2 Varieties

Let K be an algebraically closed field. We have $A_K^n = K^n$.

Definition 2.1. We say that $S \subset A_K^n$ is an algebraic set if $S = V(I)$, where I is an ideal in $K[x_1, \dots, x_n]$ and

$$V(I) = \{P \in A^n = K^n : \text{for all } f \in I, f(P) = 0\}.$$

Definition 2.2. Given a set $S \subset A^n$, we can ask for the ideal that vanish on S and take

$$I(S) := \{f \in K[x_1, \dots, x_n] : \text{for all } s \in S, f(s) = 0\}.$$

We now have functions between the sets

$$\{\text{algebraic sets}\} \text{ and } \{\text{ideal of } K[x_1, \dots, x_n]\}.$$

Definition 2.3. An affine algebraic set V is an affine variety if $I(V)$ is a prime ideal in $K[x_1, \dots, x_n]$. In particular, we observe that the quotient ring

$$K[V] = K[x_1, \dots, x_n]/I(V)$$

is an integral domain.

Definition 2.4. Let V be a variety. Then the dimension of V or $\dim V$ is the transcendence degree of $K(V)$, the field of fractions of $K[V]$, over K . Note that every nonzero element in $K[V]$ has an inverse in $K(V)$ because $K[V]$ is an integral domain.

Definition 2.5. Let V be a variety, $P \in V$, and $f_1, \dots, f_m \in \overline{K}[X]$ a set of generators for $I(V)$. Then V is *nonsingular* (or *smooth*) at P if the $m \times n$ matrix

$$\left(\frac{\partial f_i}{\partial X_j}(P) \right)_{1 \leq i \leq m, 1 \leq j \leq n}$$

has rank $n - \dim(V)$. If V is nonsingular at every point, then we say that V is nonsingular (or smooth).

Let V be given by a single nonconstant polynomial equation

$$f(X_1, \dots, X_n) = 0.$$

Then $\dim(V) = n - 1$, so $P \in V$ is a singular point if and only if

$$\frac{\partial f}{\partial X_1}(P) = \dots = \frac{\partial f}{\partial X_n}(P) = 0.$$

Since P also satisfies $f(P) = 0$, this gives $n + 1$ equations for the n coordinates of any singular point.

3 Topology on A^n

Definition 3.1. In the Zariski topology, we take the closed sets to be

$$\tau_{\text{Zariski}}(A^n) = \{\text{algebraic sets}\}.$$

We check easily that τ_{Zariski} contains $\emptyset = V(1)$ and $A^n = V(0)$. Moreover, τ_{Zariski} is stable under arbitrary intersections and finite unions.

Proof. Suppose $Y_1 = V(T_1)$ and $Y_2 = V(T_2)$. Then $Y_1 \cap Y_2 = V(T_1 T_2)$. If $Y_\alpha = V(T_\alpha)$ is any family of algebraic sets, then $\bigcap Y_\alpha = V(\bigcup T_\alpha)$. \square

Example 2. To illustrate the peculiarities of the Zariski topology, we consider the space of complex numbers \mathbb{C} . Since \mathbb{C} is algebraically closed and any ideal $I \subset \mathbb{C}[x]$ is principal, we have

$$V(I) = V(\langle f \rangle) = \{z \in \mathbb{C} \mid f(z) = 0\}, \text{ which means } |V(I)| = \deg f.$$

Then a set in \mathbb{C} is finite if and only if it is closed. In particular, this topology is not Hausdorff because any open set is infinite so given any $x_1 \neq x_2$, we must have

$$u(x_1) \cap u(x_2) \neq \emptyset.$$

In more intuitive terms, the open sets here are “too big” to separate points.

Definition 3.2. A nonempty subset Y of a topological space X is *irreducible* if it cannot be expressed as the union $Y = Y_1 \cup Y_2$ of two proper subsets, each one of which is closed in Y . The empty set is not considered to be irreducible.

Example 3. Any nonempty open subset of an irreducible space is irreducible and dense.

Proof. Let $U \subset Y$ be a non-empty open subset. We check first that $\overline{U} = Y$, otherwise $Y = U^c \cup \overline{U}$, which gives a contradiction. Now assume by way of contradiction that $U = A \cup B$. Then $Y = \overline{U} = \overline{A \cup B}$. If we take $Y = \overline{A}$ without loss of generality, we get that the closure of A in U is A . Then

$$A = \overline{A} \cap U = Y \cap U = U,$$

so U is also irreducible. □

Example 4. If Y is an irreducible subset of X , then its closure \overline{Y} in X is also irreducible.

Proof. Assume by way of contradiction that Y is irreducible but \overline{Y} is not. Then we can write $\overline{Y} = A \cup B$ for A, B proper, closed subsets. We get

$$Y = (A \cap Y) \cup (B \cap Y),$$

which are respectively closed in Y . □

We now describe some of the properties of the function which maps ideals to algebraic sets and the function which maps algebraic sets to ideals.

Theorem 3.3. (*Hilbert's Nullstellensatz*) Let k be an algebraically closed field, let \mathfrak{a} be an ideal in $A = k[x_1, \dots, x_n]$, and let $f \in A$ be a polynomial which vanishes at all points of $V(\mathfrak{a})$. Then $f^r \in \mathfrak{a}$ for some integer $r > 0$.

Proposition 3.4. (a) If $T_1 \subset T_2$ are subsets of A , then $V(T_1) \supset V(T_2)$.

(b) If $Y_1 \subset Y_2$ are subsets of \mathbb{A}^n , then $I(Y_1) \supset I(Y_2)$.

(c) For any two subsets Y_1, Y_2 of \mathbb{A}^n , we have $I(Y_1 \cup Y_2) = I(Y_1) \cap I(Y_2)$.

(d) For any ideal $\mathfrak{a} \subset A$, $I(V(\mathfrak{a})) = \sqrt{\mathfrak{a}}$, the radical of \mathfrak{a} .

(e) For any subset $Y \subset \mathbb{A}^n$, $V(I(Y)) = \overline{Y}$, the closure of Y .

Proof. (d) is a consequence of Hilbert's Nullstellensatz. To prove (e), we note that $Y \subset V(I(Y))$, which is a closed set, which implies $\overline{Y} \subset V(I(Y))$. Conversely, let W be any closed set containing Y . Then $W = V(\mathfrak{a})$ for some ideal \mathfrak{a} . So $V(\mathfrak{a}) \supset Y$ and by (b), $IV(\mathfrak{a}) \subset I(Y)$. But we must have $\mathfrak{a} \subset IV(\mathfrak{a})$, so by (a), we have $W = V(\mathfrak{a}) \supset VI(Y)$. Hence we conclude that $VI(Y) = \overline{Y}$. \square

Corollary 3.5. *There is a one-to-one inclusion-reversing correspondence between algebraic sets in \mathbb{A}^n and radical ideals, given by $Y \mapsto I(Y)$ and $\mathfrak{a} \mapsto V(\mathfrak{a})$. Furthermore, an algebraic set is irreducible if and only if its ideal is a prime ideal.*

Proof. If Y is irreducible, we show that $I(Y)$ is prime. Suppose that $fg \in I(Y)$, then $Y \subset V(fg) = V(f) \cup V(g)$. Thus $Y = (Y \cap V(f)) \cup (Y \cap V(g))$, both being closed subsets of Y . Since Y is irreducible, we have either $Y = Y \cap V(f)$, in which case $Y \subset V(f)$ or $Y \subset V(g)$. Hence either $f \in I(Y)$ or $g \in I(Y)$.

Conversely, let \mathfrak{p} be a prime ideal, and suppose that $V(\mathfrak{p}) = Y_1 \cup Y_2$. Then $\mathfrak{p} = I(Y_1) \cap I(Y_2)$, so either $\mathfrak{p} = I(Y_1)$ or $\mathfrak{p} = I(Y_2)$. Thus $V(\mathfrak{p}) = Y_1$ or Y_2 , which means it is irreducible. \square

For any subset $V \subset \mathbb{A}^n$, we can define a topology on V by taking the subspace topology, i.e. $U \subset V$ is open if and only if $U = K \cap V$ for some open K in \mathbb{A}^n . We can thus extend the Zariski topology to the n th projective space

$$P_{K^n}^n = (K^{n+1} - \{0\})/K^\times.$$

However, we notice here that for an algebraic set

$$V(f) = \{P \in \mathbb{P}^n \mid f(P) = 0\},$$

to be well-defined, the function f must satisfy

$$f(x_0, x_1, \dots, x_n) = 0 \iff f(\lambda x_0, \lambda x_1, \dots, \lambda x_n) = 0.$$

Hence, we must impose the additional restriction that f is a homogeneous polynomial of degree n .

4 Weierstrass Equations

Definition 4.1. We define an elliptic curve in K by the following equation

$$y^2 + a_1xy + a_3y = x^3 + a_2x^2 + a_4x + a_6, \text{ where } a_i \in K. \quad (4.1)$$

This is a cubic equation, whose solutions lie in $\mathbb{A}^2 = K^2$.

Given a polynomial $f \in K[x, y]$, we can homogenize it by taking

$$z^3 f\left(\frac{x}{z}, \frac{y}{z}\right) = zy^2 + a_1xyz + a_3yz^2 - x^3 - a_2x^2z - a_4xz^2 - a_6z^3.$$

The solutions to this equation now lie in \mathbb{P}^2 . Here $O = [0, 1, 0]$ is the base point.

If $\text{char}(\overline{K}) \neq 2$, then we can simplify the equation by completing the square. The substitution

$$y \mapsto \frac{1}{2}(y - a_1x - a_3)$$

gives an equation of the form

$$E : y^2 = 4x^3 + b_2x^2 + 2b_4x + b_6,$$

where $b_2 = a_1^2 + 4a_2$, $b_4 = 2a_4 + a_1a_3$, $b_6 = a_3^2 + 4a_6$. We also define the following quantities

$$b_8 = a_1^2a_6 + 4a_2a_6 - a_1a_3a_4 + a_2a_3^2 - a_4^2,$$

$$c_4 = b_2^2 - 24b_4,$$

$$c_6 = -b_2^3 + 36b_2b_4 - 216b_6,$$

$$\Delta = -b_2^2b_8 - 8b_4^3 - 27b_6^2 + 9b_2b_4b_6,$$

$$j = c_4^3/\Delta,$$

$$\omega = \frac{dx}{2y + a_1x + a_3} = \frac{dy}{3x^2 + 2a_2x + a_4 - a_1y}.$$

These satisfy the relations

$$4b_8 = b_2b_6 - b_4^2 \text{ and } 1728\Delta = c_4^3 - c_6^2.$$

If further $\text{char}(\overline{K}) \neq 2, 3$, then the substitution

$$(x, y) \mapsto \left(\frac{x - 3b_2}{36}, \frac{y}{108}\right),$$

eliminates the x^2 term, yielding the simpler equation

$$E : y^2 = x^3 - 27c_4x - 54c_6.$$

Definition 4.2. The quantity Δ is the *discriminant* of the Weierstrass equation, the quantity j is the j -invariant of the elliptic curve, and ω is the invariant differential associated to the Weierstrass equation.

Let $P = (x_0, y_0)$ be a singular point on the elliptic curve satisfying the Weierstrass equation. We have

$$\frac{\partial f}{\partial x}(P) = \frac{\partial f}{\partial y}(P) = 0.$$

It follows that there are $\alpha, \beta \in \overline{K}$ such that the Taylor series expansion of $f(x, y)$ at P has the form

$$f(x, y) - f(x_0, y_0) = ((y - y_0) - \alpha(x - x_0))((y - y_0) - \beta(x - x_0)) - (x - x_0)^3.$$

Definition 4.3. The singular point P is a *node* if $\alpha \neq \beta$. In this case, the lines

$$y - y_0 = \alpha(x - x_0) \text{ and } y - y_0 = \beta(x - x_0)$$

are the *tangent lines* at P . Conversely, if $\alpha = \beta$, then we say that P is a *cusp*, in which case the *tangent line* at P is given by

$$y - y_0 = \alpha(x - x_0).$$

Here, we mention that the Weierstrass equation for an elliptic curve may not necessarily be unique. Assuming that the line at infinity, i.e. the line $Z = 0$ in \mathbb{P}^2 is required to intersect E only at the one point $[0, 1, 0]$. We will see that the only change of variables fixing $[0, 1, 0]$ and preserving the Weierstrass form of the equation

$$x = u^2 x' r \text{ and } y = u^3 y' + u^2 s x' + t,$$

where $u, r, s, t \in \overline{K}$ and $u \neq 0$. The coefficients and associated quantities for the new equation are compiled in Table 3.1 of [3]. Here, we check that the j -invariant does not depend on the equation. If the characteristic of K is not 2 or 3, our elliptic curve(s) have Weierstrass equation(s) of the form

$$E : y^2 = x^3 + Ax + B.$$

Associated to this equation are the quantities

$$\Delta = -16(4A^3 + 27B^2) \text{ and } j = -1728 \frac{(4A)^3}{\Delta}.$$

The only change of variables preserving this form of the equation is

$$x = u^2 x' \text{ and } y = u^3 y' \text{ for some } u \in \overline{K}^*$$

with $u^4 A' = A, u^6 B' = B, u^{12} \Delta' = \Delta$.

Proposition 4.4. (a) *The curve given by a Weierstrass equation satisfies:*

- (i) *It is nonsingular if and only if $\Delta \neq 0$.*
- (ii) *It has a node if and only if $\Delta = 0$ and $c_4 \neq 0$.*
- (iii) *It has a cusp if and only if $\Delta = c_4 = 0$.*

In cases (ii) and (iii), there is only the one singular point.

(b) *Two elliptic curves are isomorphic over \overline{K} if and only if they both have the same j -invariant.*

(c) *Let $j_0 \in \overline{K}$. There exists an elliptic curve defined over $K(j_0)$ whose j -invariant is equal to j_0 .*

Proof. (a) Let E be given by the Weierstrass equation

$$E : f(x, y) = y^2 + a_1xy + a_3y - x^3 - a_2x^2 - a_4x - a_6 = 0.$$

Our first goal is to show that the point at infinity is never singular. When we look at the homogeneous equation

$$F(X, Y, Z) = Y^2Z + a_1XYZ + a_3YZ^2 - X^3 - a_2X^2Z - a_4XZ^2 - a_6Z^3 = 0$$

and at the point $O = [0, 1, 0]$. Since

$$\frac{\partial F}{\partial Z}(O) = 1 \neq 0,$$

we see that O is a nonsingular point of E .

Next suppose that E is singular, say at $P_0 = (x_0, y_0)$. The substitution

$$x = x' + x_0 \text{ and } y = y' + y_0$$

leave Δ and c_4 invariant, so we assume without loss of generality that E is singular at $(0, 0)$. Then

$$a_6 = f(0, 0) = 0, \quad a_4 = \frac{\partial f}{\partial x}(0, 0) = 0, \quad a_3 = \frac{\partial f}{\partial y}(0, 0) = 0,$$

so the equation for E takes the form

$$E : f(x, y) = y^2 + a_1xy - a_2x^2 - x^3 = 0.$$

This equation has the associated quantities

$$c_4 = (a_1^2 + 4a_2)^2 \text{ and } \Delta = 0.$$

By definition, E has a node (respectively cusp) at $(0, 0)$ if the quadratic form $y^2 + a_1xy - a_2x^2$ has distinct (respectively equal) factors, which occurs if and only if the discriminant satisfies

$$a_1^2 + 4a_2 \neq (\text{respectively } =) 0.$$

To complete the proof of (i)-(iii), it remains to show that if E is nonsingular, then $\Delta \neq 0$. To simplify the computation, we assume that $\text{char}(K) \neq 2$ and consider a Weierstrass equation of the form

$$E : y^2 = 4x^3 + b_2x^2 + 2b_4x + b_6.$$

The curve E is singular if and only if there is a point $(x_0, y_0) \in E$ satisfying

$$2y_0 = 12x_0^2 + 2b_2x_0 + 2b_4 = 0.$$

In other words, the singular points are exactly the points of the form $(x_0, 0)$ such that x_0 is a double root of the cubic polynomial $4x^3 + b_2x^2 + 2b_4x + b_6$. This polynomial has a double

root if and only if its discriminant, which equals 16Δ , vanishes. This completes the proof of (i)-(iii). Further, since a cubic polynomial cannot have two double roots, E has at most one singular point.

(b) If two elliptic curves are isomorphic, then the transformation formulas show that they have the same j -invariant. For the converse, we will assume that $\text{char}(K) \geq 5$. Let E and E' be elliptic curves with the same j -invariant, say with Weierstrass equations

$$\begin{aligned} E : y^2 &= x^3 + Ax + B, \\ E' : y'^2 &= x'^3 + A'x' + B'. \end{aligned}$$

Then the assumption that $j(E) = j(E')$ means that

$$\frac{(4A)^3}{4A^3 + 27B^2} = \frac{(4A')^3}{4A'^3 + 27B'^2},$$

which yields $A^3B'^2 = A'^3B^2$. We look for an isomorphism of the form $(x, y) = (u^2x', u^3y')$ and consider three cases:

1. $A = 0 (j = 0)$. Then $B \neq 0$, since $\Delta \neq 0$ so $A' = 0$, and we obtain an isomorphism using $u = (B/B')^{1/6}$.
2. $B = 0 (j = 1728)$. Then $A \neq 0$, so $B' = 0$ and we take $u = (A/A')^{1/4}$.
3. $AB \neq 0 (j \neq 0, 1728)$. Then $A'B' \neq 0$, since if one of them were 0, then both of them would be 0, contradicting $\Delta' \neq 0$. Taking $u = (A/A')^{1/4} = (B/B')^{1/6}$ gives the desired isomorphism.

(c) Assume that $j_0 \neq 0, 1728$ and consider the curve

$$E : y^2 + xy = x^3 - \frac{36}{j_0 - 1728}x - \frac{1}{j_0 - 1728}.$$

We then get

$$\Delta = \frac{j_0^3}{(j_0 - 1728)^3} \text{ and } j = j_0.$$

For the cases $j = 0, 1728$, we take

$$E : y^2 + y = x^3, \Delta = -27, \text{ and } E : y^2 = x^3 + x, \Delta = -64$$

respectively. □

5 The Group Law

Let E be an elliptic curve given by a Weierstrass equation. Thus $E \subset \mathbb{P}^2$ consists of the points $P = (x, y)$ satisfying the Weierstrass equation, together with the point $O = [0, 1, 0]$ at infinity. Let $L \subset \mathbb{P}^2$ be a line. Then, since the equation has degree three, the line L intersects E at exactly three points, say P, Q, R . Bezout's theorem tells us that $L \cap E$ consists of exactly three points (taken with multiplicities).

We define a composition law \oplus on E by the following rule:

Definition 5.1. (Composition Law) Let $P, Q \in E$, let L be a line through P and Q (if $P = Q$, let L be the tangent line to E at P) and let R be the third point of intersection of L with E . Let L' be the line through R and O . Then L' intersects E at R, O , and a third point. We denote that third point by $P \oplus Q$.

Proposition 5.2. *The composition law has the following properties:*

(a) *If a line L intersects E at the (not necessarily distinct) points P, Q, R , then*

$$(P \oplus Q) \oplus R = O.$$

(b) *$P \oplus O = P$ for all $P \in E$.*

(c) *$P \oplus Q = Q \oplus P$ for all $P, Q \in E$.*

(d) *Let $P \in E$. There is a point of E , denoted by $\ominus P$, satisfying*

$$P \oplus (\ominus P) = O.$$

(e) *Let $P, Q, R \in E$. Then*

$$(P \oplus Q) \oplus R = P \oplus (Q \oplus R).$$

In other words, the composition law makes E into an abelian group with identity element O .

(f) *Suppose that E is defined over K . Then*

$$E(K) = \{(x, y) \in K^2 : y^2 + a_1xy + a_3y = x^3 + a_2x^2 + a_4x + a_6\} \cup \{O\}$$

is a subgroup of E .

Proof. (a) follows from the Composition Law. (b) Taking $Q = O$, we see that the lines L and L' coincide. The former intersects E at P, O, R and the latter at $R, O, P \oplus O$ so $P \oplus O = P$. (c) The construction of $P \oplus Q$ is symmetric. (d) Let the line through P and Q also intersect E at R . Then using (a) and (b), we find that

$$O = (P \oplus O) \oplus R = P \oplus R.$$

(f) The third point of intersection has coordinates given by a rational combination of the coordinates of the coefficients of the line and of E . \square

To conclude, we derive the explicit formulas for the group operations on E . Let E be an elliptic curve given by a Weierstrass equation

$$F(x, y) = y^2 + a_1xy + a_3y - x^3 - a_2x^2 - a_4x - a_6 = 0,$$

and let $P_0 = (x_0, y_0) \in E$. In order to calculate $\ominus P_0$, we take the line L through P_0 and O and find its third point of intersection with E . The line L is given by

$$L : x - x_0 = 0.$$

Substituting this into the equation for E , we see that the quadratic polynomial $F(x_0, y)$ has roots y_0 and y'_0 where $-P = (x_0, y'_0)$. Writing out

$$F(x_0, y) = c(y - y_0)(y - y'_0)$$

and equating the coefficients of y^2 gives $c = 1$, and similarly equating the coefficients of y gives $y'_0 = -y_0 - a_1x_0 - a_3$. This yields

$$-P_0 = -(x_0, y_0) = (x_0, -y_0 - a_1x_0 - a_3).$$

Now let $P_1 = (x_1, y_1)$ and $P_2 = (x_2, y_2)$ be points of E . If $x_1 = x_2$ and $y_1 + y_2 + a_1x_2 + a_3 = 0$, then we have already shown that $P_1 + P_2 = O$. Otherwise the line L through P_1 and P_2 has an equation of the form

$$L : y = \lambda x + \nu;$$

formulas for λ and ν are given below. Substituting the equation of L into the equation of E , we see that $F(x, \lambda x + \nu)$ has roots x_1, x_2, x_3 , where $P_3 = (x_3, y_3)$ is the third point of $L \cap E$. We get $P_1 + P_2 + P_3 = O$. We write out

$$F(x, \lambda x + \nu) = c(x - x_1)(x - x_2)(x - x_3)$$

and equate coefficients. The coefficient of x^3 gives $c = -1$, and then the coefficient of x^2 yields

$$x_1 + x_2 + x_3 = \lambda^2 + a_1\lambda - a_2.$$

This gives a formula for x_3 , and substituting into the equation of L gives the value of $y_3 = \lambda x_3 + \nu$. Finally, to find $P_1 + P_2 = -P_3$, we apply the negation formula to P_3 . We summarize these steps with the following algorithm.

Theorem 5.3. (*Group Law Algorithm*) *Let E be an elliptic curve given by a Weierstrass equation*

$$E : y^2 + a_1xy + a_3y = x^3 + a_2x^2 + a_4x + a_6.$$

(a) *Let $P_0 = (x_0, y_0)$. Then*

$$-P_0 = (x_0, -y_0 - a_1x_0 - a_3).$$

- (b) Next let $P_1 + P_2 = P_3$. If $x_1 = x_2$ and $y_1 + y_2 + a_1x_2 + a_3 = 0$, then $P_1 + P_2 = O$. Otherwise, if $x_1 = x_2$, take

$$\lambda = \frac{3x_1^2 + 2a_2x_1 + a_4 - a_1y_1}{2y_1 + a_1x_1 + a_3}, \nu = \frac{-x_1^3 + a_4x_1 + 2a_6 - a_3y_1}{2y_1 + a_1x_1 + a_3}.$$

Then $y = \lambda x + \nu$ is the line through P_1 and P_2 , or tangent to E if $P_1 = P_2$.

- (c) With notation as in (b), $P_3 = P_1 + P_2$ has coordinates

$$\begin{aligned} x_3 &= \lambda^2 + a_1\lambda - a_2 - x_1 - x_2, \\ y_3 &= -(\lambda + a_1)x_3 - \nu - a_3. \end{aligned}$$

- (d) As special cases of (c), we have for $P_1 \neq \pm P_2$,

$$x(P_1 + P_2) = \left(\frac{y_2 - y_1}{x_2 - x_1} \right)^2 + a_1 \left(\frac{y_2 - y_1}{x_2 - x_1} \right) - a_2 - x_1 - x_2,$$

and the duplication formula for $P = (x, y) \in E$

$$x(P + P) = \frac{x^4 - b_4x^2 - 2b_6x - b_8}{4x^3 + b_2x^2 + 2b_4x + b_6},$$

where b_2, b_4, b_6, b_8 are the polynomials in the a_i 's.

References

- [1] Robin Hartshorne (1977) *Algebraic Geometry*, Springer Science+Business Media, Inc.
- [2] Joseph H. Silverman, John T. Tate (2015) *Rational Points on Elliptic Curves*, Springer International Publishing Switzerland.
- [3] Joseph H. Silverman (2009) *The Arithmetic of Elliptic Curves*, Springer Science+Business Media, Inc.